coq_alt/Props.v
@@ -1,0 +1,69 @@
+Set Implicit Arguments.
+Require Import Strings.String CSC.Util.
+
+(** * This file defines the trace properties of the paper. *)
+
+Variant ControlTag : Type :=
+| CCtx
+| CComp
+.
+Variant SecurityTag : Type :=
+| SLock
+| SUnlock
+.
+Variant PreEvent : Type :=
+| Alloc (l : loc) (n : nat)
+| Use (l : loc) (n : nat)
+| Dealloc (l : loc)
+| Branch (n : nat)
+| Binop (n : nat)
+.
+Inductive Event : Type :=
+| Aborted
+| PreEv (a__b : PreEvent) (t : ControlTag) (σ : SecurityTag)
+.
+#[export]
+Instance MGT__Instance : TraceParams := {
+  Ev := Event ;
+  string_of_event := fun _ => ""%string ;
+}.
+
+(** Trace property definitions *)
+
+(** Safety Property *)
+Definition prop := tracepref -> Prop.
+
+(** Temporal Memory Safety *)
+Definition tms : prop := fun (As : tracepref) =>
+                           (forall l n t t' σ σ', before (PreEv (Alloc l n) t σ) (PreEv (Dealloc l) t' σ') As)
+                         /\ (forall l n m t t' σ σ', ~before (PreEv (Use l n) t σ) (PreEv (Alloc l m) t' σ') As)
+                         /\ (forall l n t t' σ σ', ~before (PreEv (Dealloc l) t σ) (PreEv (Use l n) t' σ') As)
+.
+(** Spatial Memory Safety *)
+Definition sms : prop := fun (As : tracepref) =>
+                           forall l n m t t' σ σ', before (PreEv (Alloc l m) t σ) (PreEv (Use l n) t' σ') As ->
+                                              n < m
+.
+(** Strict Cryptographic Constant Time *)
+Fixpoint no_secrets (As : tracepref) : tracepref :=
+  match As with
+  | List.nil => List.nil
+  | List.cons a As =>
+    match a with
+    | Aborted => List.cons Aborted (no_secrets As)
+    | PreEv a__b t SLock => no_secrets As
+    | PreEv a__b t SUnlock => List.cons a (no_secrets As)
+    end
+  end
+.
+Definition sCCT : prop := fun (As : tracepref) =>
+                            As = no_secrets As
+.
+
+Module PropNotations.
+  Declare Scope PropNotationsScope.
+  Delimit Scope PropNotationsScope with propnotationsscope.
+
+  Notation "e '∈' π" := (π e) (at level 81, π at next level) : PropNotationsScope.
+  Notation "π1 '∩' π2" := ((fun (t : tracepref) => t ∈ π1 /\ t ∈ π2)%propnotationsscope) (at level 81, π2 at next level, left associativity) : PropNotationsScope.
+End PropNotations.
